Add test for Set.Empty

rocq/ZF/Meta/Decl/Set/Empty.v
@@ -1,8 +1,8 @@
 Require Import Coq.Lists.List.
 Require Import Coq.Strings.String.
 
+Require Import ZF.Meta.DeclP.
 Require Import ZF.Meta.DeclT.
-Require Import ZF.Meta.Env.
 Require Import ZF.Meta.Env.
 Require Import ZF.Meta.SyntaxT.
 Require Import ZF.Meta.SyntaxP.
@@ -11,18 +11,218 @@ Require Import ZF.Meta.Ty.
 Import ListNotations.
 Open Scope string_scope.
 
+Require Import ZF.Meta.Decl.Class.Empty.
+Require Import ZF.Meta.Decl.Class.Equiv.
+Require Import ZF.Meta.Decl.Set.Incl.
+Require Import ZF.Meta.Decl.Set.OrdPair.
+Require Import ZF.Meta.Decl.Set.Pair.
+Require Import ZF.Meta.Decl.Set.Single.
+
 (* empty : U.                                                                   *)
 Definition empty : DeclT :=
-  {| paraT := [];
-     resT  := TySet;
-     bodyT := HoleT TySet |}.
+  {| paraT := []
+  ;  resT  := TySet
+  ;  bodyT := FromC (IdentT (Name.qualified "CEM" "empty") (args []))
+  |}.
 
-Definition imports : Env := Env.empty.
+(* toClass empty is equivalent to the empty class.                              *)
+Definition ToClass : DeclP :=
+  let concl :=
+    IdentT (Name.local "equiv")
+      (args
+        [ IdentT (Name.local "toClass")
+            (args [IdentT (Name.local "empty") (args [])])
+        ; IdentT (Name.qualified "CEM" "empty") (args [])
+        ])
+  in
+    {| paraP  := []
+    ;  conclP := concl
+    ;  bodyP  := HoleP concl
+    |}.
 
-Definition exports : Env := Env.fromListT
-  [ (Name.local "empty", empty)
+(* forall x, x :< empty <-> False.                                              *)
+Definition Charac : DeclP :=
+  let concl :=
+    All
+      (Iff
+        (Elem (Var 0) (IdentT (Name.local "empty") (args [])))
+        Bot)
+  in
+    {| paraP  := []
+    ;  conclP := concl
+    ;  bodyP  := HoleP concl
+    |}.
+
+(* forall a, Incl empty a.                                                      *)
+Definition IsIncl : DeclP :=
+  let concl :=
+    IdentT (Name.local "Incl")
+      (args [IdentT (Name.local "empty") (args []); Var 0])
+  in
+    {| paraP  := [TySet]
+    ;  conclP := concl
+    ;  bodyP  := HoleP concl
+    |}.
+
+(* forall x, not x :< empty.                                                    *)
+Definition NoElem : DeclP :=
+  let concl :=
+    All
+      (Not (Elem (Var 0) (IdentT (Name.local "empty") (args []))))
+  in
+    {| paraP  := []
+    ;  conclP := concl
+    ;  bodyP  := HoleP concl
+    |}.
+
+(* forall a, a <> empty iff exists x, x :< a.                                   *)
+Definition HasElem : DeclP :=
+  let concl :=
+    Iff
+      (NotEq (Var 0) (IdentT (Name.local "empty") (args [])))
+      (Ex (Elem (Var 0) (Var 1)))
+  in
+    {| paraP  := [TySet]
+    ;  conclP := concl
+    ;  bodyP  := HoleP concl
+    |}.
+
+(* forall a, a = empty iff not exists x, x :< a.                                *)
+Definition HasNoElem : DeclP :=
+  let concl :=
+    Iff
+      (SyntaxT.Equal (Var 0) (IdentT (Name.local "empty") (args [])))
+      (Not (Ex (Elem (Var 0) (Var 1))))
+  in
+    {| paraP  := [TySet]
+    ;  conclP := concl
+    ;  bodyP  := HoleP concl
+    |}.
+
+(* forall a, no element belongs to a -> a = empty.                              *)
+Definition WhenNoElem : DeclP :=
+  let concl :=
+    Imp
+      (All (Not (Elem (Var 0) (Var 1))))
+      (SyntaxT.Equal (Var 0) (IdentT (Name.local "empty") (args [])))
+  in
+    {| paraP  := [TySet]
+    ;  conclP := concl
+    ;  bodyP  := HoleP concl
+    |}.
+
+(* forall a b, pair a b <> empty.                                               *)
+Definition PairIsNotEmpty : DeclP :=
+  let concl :=
+    NotEq
+      (IdentT (Name.local "pair") (args [Var 1; Var 0]))
+      (IdentT (Name.local "empty") (args []))
+  in
+    {| paraP  := [TySet; TySet]
+    ;  conclP := concl
+    ;  bodyP  := HoleP concl
+    |}.
+
+(* forall x y, ordPair x y <> empty.                                            *)
+Definition OrdPairIsNotEmpty : DeclP :=
+  let concl :=
+    NotEq
+      (IdentT (Name.local "ordPair") (args [Var 1; Var 0]))
+      (IdentT (Name.local "empty") (args []))
+  in
+    {| paraP  := [TySet; TySet]
+    ;  conclP := concl
+    ;  bodyP  := HoleP concl
+    |}.
+
+(* forall a, single a <> empty.                                                 *)
+Definition SingletonIsNotEmpty : DeclP :=
+  let concl :=
+    NotEq
+      (IdentT (Name.local "single") (args [Var 0]))
+      (IdentT (Name.local "empty") (args []))
+  in
+    {| paraP  := [TySet]
+    ;  conclP := concl
+    ;  bodyP  := HoleP concl
+    |}.
+
+(* forall a, a = empty iff toClass a is the empty class.                        *)
+Definition EmptyToClass : DeclP :=
+  let concl :=
+    Iff
+      (SyntaxT.Equal (Var 0) (IdentT (Name.local "empty") (args [])))
+      (IdentT (Name.local "equiv")
+        (args
+          [ IdentT (Name.local "toClass") (args [Var 0])
+          ; IdentT (Name.qualified "CEM" "empty") (args [])
+          ]))
+  in
+    {| paraP  := [TySet]
+    ;  conclP := concl
+    ;  bodyP  := HoleP concl
+    |}.
+
+(* forall a, a <> empty iff toClass a is not the empty class.                   *)
+Definition NotEmptyToClass : DeclP :=
+  let concl :=
+    Iff
+      (NotEq (Var 0) (IdentT (Name.local "empty") (args [])))
+      (Not
+        (IdentT (Name.local "equiv")
+          (args
+            [ IdentT (Name.local "toClass") (args [Var 0])
+            ; IdentT (Name.qualified "CEM" "empty") (args [])
+            ])))
+  in
+    {| paraP  := [TySet]
+    ;  conclP := concl
+    ;  bodyP  := HoleP concl
+    |}.
+
+(* forall a, Incl a empty -> a = empty.                                         *)
+Definition WhenIncl : DeclP :=
+  let concl :=
+    Imp
+      (IdentT (Name.local "Incl")
+        (args [Var 0; IdentT (Name.local "empty") (args [])]))
+      (SyntaxT.Equal (Var 0) (IdentT (Name.local "empty") (args [])))
+  in
+    {| paraP  := [TySet]
+    ;  conclP := concl
+    ;  bodyP  := HoleP concl
+    |}.
+
+(* Environment.                                                                 *)
+
+Definition imports : Env := Env.unions
+  [ Env.qualifyAs "CEM" Empty.exports
+  ; Env.unqualify Equiv.exports
+  ; Env.unqualify Incl.exports
+  ; Env.unqualify OrdPair.exports
+  ; Env.unqualify Pair.exports
+  ; Env.unqualify Single.exports
+  ].
+
+Definition exports : Env := Env.unions
+  [ Env.fromListT
+      [ (Name.local "empty", empty)
+      ]
+  ; Env.fromListP
+      [ (Name.local "ToClass"           , ToClass)
+      ; (Name.local "Charac"            , Charac)
+      ; (Name.local "IsIncl"            , IsIncl)
+      ; (Name.local "NoElem"            , NoElem)
+      ; (Name.local "HasElem"           , HasElem)
+      ; (Name.local "HasNoElem"         , HasNoElem)
+      ; (Name.local "WhenNoElem"        , WhenNoElem)
+      ; (Name.local "PairIsNotEmpty"    , PairIsNotEmpty)
+      ; (Name.local "OrdPairIsNotEmpty" , OrdPairIsNotEmpty)
+      ; (Name.local "SingletonIsNotEmpty", SingletonIsNotEmpty)
+      ; (Name.local "EmptyToClass"      , EmptyToClass)
+      ; (Name.local "NotEmptyToClass"   , NotEmptyToClass)
+      ; (Name.local "WhenIncl"          , WhenIncl)
+      ]
   ].
 
 Definition env : Env := Env.union imports exports.
-
-
